Nlp/Syntax.lean
@@ -1,5 +1,6 @@
 import Nlp.Syntax.Tree
 import Nlp.Syntax.TreeLemmas
 import Nlp.Syntax.AnnTree
+import Nlp.Syntax.NamedTree
 
 /-! Constituency syntax data structures. -/
