NlpTests/Syntax.lean
@@ -1,3 +1,4 @@
 import NlpTests.Syntax.Tree
 import NlpTests.Syntax.TreeLemmas
 import NlpTests.Syntax.AnnTree
+import NlpTests.Syntax.NamedTree
